Add aeq equivalence attributes

src/aeq/id.lean
@@ -11,11 +11,12 @@ namespace aeq ------------------------------------------------------------------
 
 variables {V : Type} [decidable_eq V] -- Type of variable names
 variables {vs : Type → Type} [vset vs V] -- Type of variable name sets
+variables {X : vs V} -- Variable name sets
 
 -- Identity `aeq` with an implicit `vset`.
 @[inline, reducible]
 protected
-def id {X : vs V} : exp X → exp X → Prop :=
+def id : exp X → exp X → Prop :=
   aeq (vrel.id X)
 
 -- Notation for `aeq.id`.
@@ -25,26 +26,32 @@ namespace id -------------------------------------------------------------------
 -- Paper: Corollary 3
 
 -- Reflexivity of `aeq.id`
+@[refl]
 protected
-theorem refl (X : vs V) : reflexive (aeq (vrel.id X)) :=
+theorem refl : ∀ (e : exp X), aeq (vrel.id X) e e :=
   aeq.refl
 
 -- Symmetry of `aeq.id`
+@[symm]
 protected
-theorem symm (X : vs V) : symmetric (aeq (vrel.id X)) :=
-  λ e₁ e₂ a,
-  map.simple (λ x₁ x₂, vrel.inv.of_id) (aeq.symm a)
+theorem symm ⦃e₁ e₂ : exp X⦄
+: aeq (vrel.id X) e₁ e₂ → aeq (vrel.id X) e₂ e₁ :=
+  λ a, map.simple (λ x₁ x₂, vrel.inv.of_id) (aeq.symm a)
 
 -- Transitivity of `aeq.id`
+@[trans]
 protected
-theorem trans (X : vs V) : transitive (aeq (vrel.id X)) :=
-  λ e₁ e₂ e₃ a₁ a₂,
-  map.simple (λ x₁ x₂, vrel.id.of_comp) (aeq.trans a₁ a₂)
+theorem trans ⦃e₁ e₂ e₃ : exp X⦄
+: aeq (vrel.id X) e₁ e₂ → aeq (vrel.id X) e₂ e₃ → aeq (vrel.id X) e₁ e₃ :=
+  λ a₁ a₂, map.simple (λ x₁ x₂, vrel.id.of_comp) (aeq.trans a₁ a₂)
 
 -- Equivalence
 protected
 theorem equiv (X : vs V) : equivalence (aeq (vrel.id X)) :=
-  mk_equivalence (aeq (vrel.id X)) (id.refl X) (id.symm X) (id.trans X)
+  mk_equivalence (aeq (vrel.id X))
+    (@id.refl _ _ _ _ X)
+    (@id.symm _ _ _ _ X)
+    (@id.trans _ _ _ _ X)
 
 -- Setoid
 instance setoid (X : vs V) : setoid (exp X) :=
